SoftwareFoundations/SfLib/Smallstep.v
@@ -1,0 +1,458 @@
+(**** Smallstep: Small-step Operational Semantics ****)
+
+Require Export Imp.
+
+(*** Relations ***)
+
+Definition relation (X : Type) := X -> X -> Prop.
+
+(*** A Toy Language ***)
+
+Inductive tm : Type :=
+| C : nat -> tm
+| P : tm -> tm -> tm.
+
+Module SimpleArith0.
+
+  Fixpoint eval (t : tm) : nat :=
+    match t with
+      | C n => n
+      | P a1 a2 => eval a1 + eval a2
+    end.
+
+End SimpleArith0.
+
+Reserved Notation " t '||' n " (at level 50, left associativity).
+
+Inductive eval : tm -> nat -> Prop :=
+| E_Const : forall n, C n || n
+| E_Plus : forall t1 t2 n1 n2, t1 || n1 -> t2 || n2 -> P t1 t2 || (n1 + n2)
+where " t '||' n " := (eval t n).
+
+Module SimpleArith1.
+
+  Reserved Notation " t '=>' t' " (at level 40).
+
+  Inductive step : tm -> tm -> Prop :=
+  | ST_PlusConstConst : forall n1 n2, P (C n1) (C n2) => C (n1 + n2)
+  | ST_Plus1 : forall t1 t1' t2, t1 => t1' -> P t1 t2 => P t1' t2
+  | ST_Plus2 : forall n1 t2 t2', t2 => t2' -> P (C n1) t2 => P (C n1) t2'
+  where " t '=>' t' " := (step t t').
+
+  Example test_step_1:
+    P (P (C 0) (C 3)) (P (C 2) (C 4)) => P (C (0 + 3)) (P (C 2) (C 4)).
+  Proof.
+    repeat constructor.
+  Qed.
+
+  Example test_step_2:
+    P (C 0) (P (C 2) (P (C 0) (C 3))) => P (C 0) (P (C 2) (C (0 + 3))).
+  Proof.
+    repeat constructor.
+  Qed.
+
+  Definition deterministic {X : Type} (R : relation X) :=
+    forall x y1 y2 : X, R x y1 -> R x y2 -> y1 = y2.
+
+  Theorem step_deterministic:
+    deterministic step.
+  Proof.
+    unfold deterministic.
+    intros x y1 y2 Hy1. generalize dependent y2.
+    induction Hy1; intros y2 Hy2.
+      (* ST_PlusConstConst *)
+      inversion Hy2.
+        (* ST_PlusConstCOnst *) reflexivity.
+        (* ST_Plus1          *) inversion H2.
+        (* ST_Plus2          *) inversion H2.
+      (* ST_Plus1 *)
+      inversion Hy2; subst.
+        (* ST_PlusConstConst *) inversion Hy1.
+        (* ST_Plus1          *) rewrite <- (IHHy1 t1'0). reflexivity. assumption.
+        (* ST_Plus2          *) inversion Hy1.
+      inversion Hy2; subst.
+        (* ST_PlusConstConst *) inversion Hy1.
+        (* ST_Plus1          *) inversion H2.
+        (* ST_Plus2          *) rewrite <- (IHHy1 t2'0). reflexivity. assumption.
+  Qed.
+
+End SimpleArith1.
+
+(** Values **)
+
+Inductive value : tm -> Prop :=
+  v_const : forall n, value (C n).
+
+Reserved Notation " t '=>' t' " (at level 40).
+
+Inductive step : tm -> tm -> Prop :=
+| ST_PlusConstConst : forall n1 n2, P (C n1) (C n2) => C (n1 + n2)
+| ST_Plus1 : forall t1 t1' t2, t1 => t1' -> P t1 t2 => P t1' t2
+| ST_Plus2 : forall v1 t2 t2', value v1 -> t2 => t2' -> P v1 t2 => P v1 t2'
+where " t '=>' t' " := (step t t').
+
+Theorem step_deterministic:
+  deterministic step.
+Proof.
+  unfold deterministic.
+  intros x y1 y2 Hy1. generalize dependent y2.
+  induction Hy1; intros y2 Hy2.
+  (* PCC *)
+    inversion Hy2; subst.
+    (* PCC *) reflexivity.
+    (* P1  *) inversion H2.
+    (* P2  *) inversion H3.
+  (* P1  *)
+    inversion Hy2; subst.
+    (* PCC *) inversion Hy1.
+    (* P1  *) rewrite <- (IHHy1 t1'0). reflexivity. assumption.
+    (* P2  *) inversion H1. subst. inversion Hy1.
+  (* P2  *)
+    inversion Hy2; subst.
+    (* PCC *) inversion Hy1.
+    (* P1  *) inversion H. subst. inversion H3.
+    (* P2  *) rewrite <- (IHHy1 t2'0). reflexivity. assumption.
+Qed.
+
+(** Strong Progress and Normal Forms **)
+
+Theorem strong_progress:
+  forall t, value t \/ (exists t', t => t').
+Proof.
+  intro t.
+  induction t.
+    (* t = C n *)
+    left. constructor.
+    (* t = P t1 t2 *)
+    right. inversion IHt1.
+      inversion IHt2.
+        inversion H. inversion H0. exists (C (n + n0)). constructor.
+        inversion H0 as [t' H1]. exists (P t1 t'). constructor.
+          apply H.
+          apply H1.
+      inversion H as [t' H0].
+        exists (P t' t2). constructor. apply H0.
+Qed.
+
+Definition normal_form {X : Type} (R : relation X) (t : X) : Prop :=
+  ~ exists t', R t t'.
+
+Lemma value_is_nf:
+  forall t, value t -> normal_form step t.
+Proof.
+  intros t H.
+  unfold normal_form. unfold not. intro G.
+  inversion H. subst.
+  inversion G.
+  inversion H0.
+Qed.
+
+Lemma nf_is_value:
+  forall t, normal_form step t -> value t.
+Proof.
+  unfold normal_form.
+  intros t H.
+  assert (G : value t \/ exists t', t => t').
+    apply strong_progress.
+  inversion G.
+    apply H0.
+    apply ex_falso_quodlibet. apply H. assumption.
+Qed.
+
+Corollary nf_same_as_value:
+  forall t, normal_form step t <-> value t.
+Proof.
+  split.
+    apply nf_is_value.
+    apply value_is_nf.
+Qed.
+
+Module Temp1.
+
+  Inductive value : tm -> Prop :=
+  | v_const : forall n, value (C n)
+  | v_funny : forall t1 n2, value (P t1 (C n2)).
+
+  Reserved Notation " t '=>' t' " (at level 40).
+
+  Inductive step : tm -> tm -> Prop :=
+  | ST_PlusConstConst : forall n1 n2, P (C n1) (C n2) => C (n1 + n2)
+  | ST_Plus1 : forall t1 t1' t2, t1 => t1' -> P t1 t2 => P t1' t2
+  | ST_Plus2 : forall v1 t2 t2', value v1 -> t2 => t2' -> P v1 t2 => P v1 t2'
+  where " t '=>' t' " := (step t t').
+
+  Lemma value_not_same_as_normal_form:
+    exists t, value t /\ ~normal_form step t.
+  Proof.
+    exists (P (C 1) (C 2)).
+    split.
+      repeat constructor.
+      intro G. apply G. exists (C 3). constructor.
+  Qed.
+
+End Temp1.
+
+Module Temp2.
+
+  Inductive value : tm -> Prop :=
+  | v_const : forall n, value (C n).
+
+  Reserved Notation " t '=>' t' " (at level 40).
+
+  Inductive step : tm -> tm -> Prop :=
+  | ST_Funny : forall n, C n => P (C n) (C 0)
+  | ST_PlusConstConst : forall n1 n2, P (C n1) (C n2) => C (n1 + n2)
+  | ST_Plus1 : forall t1 t1' t2, t1 => t1' -> P t1 t2 => P t1' t2
+  | ST_Plus2 : forall v1 t2 t2', value v1 -> t2 => t2' -> P v1 t2 => P v1 t2'
+  where " t '=>' t' " := (step t t').
+
+  Lemma value_not_same_as_normal_form:
+    exists t, value t /\ ~normal_form step t.
+  Proof.
+    exists (C 0).
+    split.
+      constructor.
+      intro G. apply G. exists (P (C 0) (C 0)). constructor.
+  Qed.
+
+End Temp2.
+
+Module Temp3.
+
+  Inductive value : tm -> Prop :=
+  | v_const : forall n, value (C n).
+
+  Reserved Notation " t '=>' t' " (at level 40).
+
+  Inductive step : tm -> tm -> Prop :=
+  | ST_PlusConstConst : forall n1 n2, P (C n1) (C n2) => C (n1 + n2)
+  | ST_Plus1 : forall t1 t1' t2, t1 => t1' -> P t1 t2 => P t1' t2
+  where " t '=>' t' " := (step t t').
+
+  Lemma value_not_same_as_normal_form:
+    exists t, ~value t /\ normal_form step t.
+  Proof.
+    exists (P (C 0) (P (C 0) (C 0))).
+    split.
+      intro G. inversion G.
+      unfold normal_form. intro G. inversion G. inversion H. subst. inversion H3.
+  Qed.
+
+End Temp3.
+
+(* Additional Exercises *)
+
+Module Temp4.
+
+  Inductive tm : Type :=
+  | ttrue : tm
+  | tfalse : tm
+  | tif : tm -> tm -> tm -> tm.
+
+  Inductive value : tm -> Prop :=
+  | v_true : value ttrue
+  | v_false : value tfalse.
+
+  Reserved Notation " t '=>' t' " (at level 40).
+
+  Inductive step : tm -> tm -> Prop :=
+  | ST_IfTrue : forall t1 t2, tif ttrue t1 t2 => t1
+  | ST_IfFalse : forall t1 t2, tif tfalse t1 t2 => t2
+  | ST_If : forall t1 t1' t2 t3, t1 => t1' -> tif t1 t2 t3 => tif t1' t2 t3
+  where " t '=>' t' " := (step t t').
+
+  Example bool_step_prop1:
+    ~ (tfalse => tfalse).
+  Proof.
+    intro G. inversion G.
+  Qed.
+
+  Example bool_step_prop2:
+    ~ (tif ttrue (tif ttrue ttrue ttrue) (tif tfalse tfalse tfalse) => ttrue).
+  Proof.
+    intro G. inversion G.
+  Qed.
+
+  Example bool_step_prop3:
+    tif (tif ttrue ttrue ttrue) (tif ttrue ttrue ttrue) tfalse 
+    =>
+    tif ttrue (tif ttrue ttrue ttrue) tfalse.
+  Proof.
+    repeat constructor.
+  Qed.
+
+  Theorem strong_progress:
+    forall t, value t \/ (exists t', t => t').
+  Proof.
+    intro t.
+    induction t.
+      left. constructor.
+      left. constructor.
+      right. inversion IHt1.
+        inversion H.
+          exists t2. constructor.
+          exists t3. constructor.
+        inversion H.
+          exists (tif x t2 t3). apply ST_If. apply H0.
+  Qed.
+
+  Theorem step_deterministic:
+    deterministic step.
+  Proof.
+    unfold deterministic.
+    intros x y1 y2 Hy1.
+    generalize dependent y2.
+    induction Hy1; intros y2 Hy2.
+      inversion Hy2; subst.
+        reflexivity.
+        inversion H3.
+      inversion Hy2; subst.
+        reflexivity.
+        inversion H3.
+      inversion Hy2; subst.
+        inversion Hy1.
+        inversion Hy1.
+        assert (t1' = t1'0).
+          apply IHHy1. apply H3.
+        rewrite H. reflexivity.
+  Qed.
+
+  Module Temp5.
+
+    Reserved Notation " t '=>' t' " (at level 40).
+
+    Inductive step : tm -> tm -> Prop :=
+    | ST_IfTrue : forall t1 t2, tif ttrue t1 t2 => t1
+    | ST_IfFalse : forall t1 t2, tif tfalse t1 t2 => t2
+    | ST_If : forall t1 t1' t2 t3, t1 => t1' -> tif t1 t2 t3 => tif t1' t2 t3
+    | ST_Shortcut : forall t1 t2 t3,
+                      value t2 -> value t3 -> t2 = t3 -> tif t1 t2 t3 => t2
+    where " t '=>' t' " := (step t t').
+
+    Theorem step_not_deterministic:
+      ~deterministic step.
+    Proof.
+    Admitted. (* FIXME *)
+
+    Theorem strong_progress:
+      forall t, value t \/ (exists t', t => t').
+    Proof.
+    Admitted. (* FIXME *)
+
+    (* Yes, any one of them. *)
+
+  End Temp5.
+
+End Temp4.
+
+(*** Multi-Step Reduction ***)
+
+(** Definitions **)
+
+(* Already in SfLib!
+
+  Inductive multi {X : Type} (R : relation X) : relation X :=
+  | multi_refl : forall (x : X), multi R x x
+  | multi_step : forall (x y z : X), R x y -> multi R y z -> multi R x z.
+
+*)
+
+Theorem mutli_R:
+  forall (X : Type) (R : relation X) (x y : X), R x y -> (multi R) x y.
+Proof.
+  intros X R x y H.
+  apply multi_step with y.
+    apply H.
+    apply multi_refl.
+Qed.
+
+Theorem multi_trans:
+  forall (X : Type) (R : relation X) (x y z : X), multi R x y -> multi R y z -> multi R x z.
+Proof.
+  intros X R x y z G H.
+  induction G.
+    assumption.
+    apply multi_step with y. assumption. apply IHG. assumption.
+Qed.
+
+Definition multistep := multi step.
+
+Notation " t '=>*' t' " := (multistep t t') (at level 40).
+
+(** Examples **)
+
+Example test_multistep_1:
+  P (P (C 0) (C 3)) (P (C 2) (C 4)) =>* C ((0 + 3) + (2 + 4)).
+Proof.
+  apply multi_step with (P (C (0 + 3)) (P (C 2) (C 4))).
+    repeat constructor.
+    apply multi_step with (P (C (0 + 3)) (C (2 + 4))).
+      repeat constructor.
+      apply multi_R.
+        constructor.
+Qed.
+
+Example test_multistep_1':
+  P (P (C 0) (C 3)) (P (C 2) (C 4)) =>* C ((0 + 3) + (2 + 4)).
+Proof.
+  eapply multi_step.
+    repeat constructor.
+    eapply multi_step.
+      apply ST_Plus2. apply v_const.
+      apply ST_PlusConstConst.
+      eapply multi_step.
+        apply ST_PlusConstConst.
+        apply multi_refl.
+Qed.
+
+Example test_multistep_2:
+  C 3 =>* C 3.
+Proof.
+  apply multi_refl.
+Qed.
+
+Example test_multistep_3:
+  P (C 0) (C 3) =>* P (C 0) (C 3).
+Proof.
+  constructor.
+Qed.
+
+Example test_multistep_4:
+  P (C 0) (P (C 2) (P (C 0) (C 3))) =>* P (C 0) (C (2 + (0 + 3))).
+Proof.
+  apply multi_step with (P (C 0) (P (C 2) (C (0 + 3)))).
+  repeat constructor.
+  apply multi_R.
+  repeat constructor.
+Qed.
+
+(** Normal Forms Again **)
+
+Definition step_normal_form := normal_form step.
+
+Definition normal_form_of (t t' : tm) := t =>* t' /\ step_normal_form t'.
+
+Theorem normal_forms_unique:
+  deterministic normal_form_of.
+Proof.
+  unfold deterministic. unfold normal_form_of.
+  intros x y1 y2 P1 P2.
+  inversion P1 as [P11 P12]; clear P1.
+  inversion P2 as [P21 P22]; clear P2.
+  generalize dependent y2.
+  induction y1; intros.
+    (* t = C n *)
+    inversion P11; subst.
+      inversion P21; subst.
+        reflexivity.
+        inversion H.
+      admit.
+    (* t = P t1 t2 *)
+    inversion P21. inversion P11.
+      subst. symmetry. apply H2.
+Admitted. (* FIXME *)
+
+
+      
+  
+                        
