SoftwareFoundations/SfLib/Types.v
@@ -1,0 +1,41 @@
+(**** Types: Type Systems ****)
+
+Require Export Smallstep.
+
+(*** More Automation ***)
+
+(** The 'auto' and 'eauto' Tactics **)
+
+Example auto_example_1:
+  forall P Q R S T U : Prop, (P -> Q) -> (P -> Q) -> (T -> R) ->
+                             (S -> T -> U) -> ((P -> Q) -> (P -> S)) -> T -> P -> U.
+Proof.
+  auto.
+Qed.
+
+Lemma auto_example_2:
+  forall P Q R : Prop, Q -> (Q -> R) -> P \/ (Q /\ R).
+Proof.
+  auto.
+Qed.
+
+Lemma auto_example_2a:
+  forall P Q R : Prop, Q -> (Q -> R) -> P \/ (Q /\ R).
+Proof.
+  auto using conj, or_introl, or_intror.
+Qed.
+
+Hint Constructors multi.
+Hint Resolve beq_id_eq beq_id_false_not_eq.
+
+(** The 'Proof with' Tactic **)
+
+(** The 'solve by inversion' Tactic **)
+
+(** The 'try solve' Tactic **)
+
+(** The 'f_equal' Tactic **)
+
+Definition amultistep st := multi (astep st).
+
+Notation " t '/' st '=>a*' t' " := (amultistep st t t') (at level 40, st at level 39).
